{-# OPTIONS --cubical --safe #-}

open import Algebra
open import Prelude
open import HITs.PropositionalTruncation
open import HITs.PropositionalTruncation.Sugar

module Algebra.Construct.Cayley {a} (mon : Monoid a) where

open Monoid mon

ğ’ : Type a
ğ’ = Î£[ f â¦‚ (ğ‘† â†’ ğ‘†) ] Ã— âˆ€ x â†’ âˆ¥ f Îµ âˆ™ x â‰¡ f x âˆ¥


âŸ¦_â‡“âŸ§ : ğ’ â†’ ğ‘†
âŸ¦ x â‡“âŸ§ = x .fst Îµ

âŸ¦_â‡‘âŸ§ : ğ‘† â†’ ğ’
âŸ¦ x â‡‘âŸ§ .fst y = x âˆ™ y
âŸ¦ x â‡‘âŸ§ .snd y = âˆ£ cong (_âˆ™ y) (âˆ™Îµ x) âˆ£

â“” : ğ’
â“” .fst x = x
â“” .snd x = âˆ£ Îµâˆ™ x âˆ£

open import Relation.Binary
open import HITs.PropositionalTruncation.Equivalence
open import Relation.Binary.Equivalence.Reasoning (trunc-equivalence (â‰¡-equivalence {A = ğ‘†}))

_âŠ™_ : ğ’ â†’ ğ’ â†’ ğ’
(x âŠ™ y) .fst z = x .fst (y .fst z)
(x âŠ™ y) .snd z =
  x .fst (y .fst Îµ) âˆ™ z     â‰‹Ë˜âŸ¨ cong (_âˆ™ z) âˆ¥$âˆ¥ (x .snd (y .fst Îµ)) âŸ©
  x .fst Îµ âˆ™ y .fst Îµ âˆ™ z   â‰¡âŸ¨ assoc (x .fst Îµ) (y .fst Îµ) z âŸ©
  x .fst Îµ âˆ™ (y .fst Îµ âˆ™ z) â‰‹âŸ¨ cong (x .fst Îµ âˆ™_) âˆ¥$âˆ¥ (y .snd z)  âŸ©
  x .fst Îµ âˆ™ y .fst z       â‰‹âŸ¨ x .snd (y .fst z) âŸ©
  x .fst (y .fst z) âˆ

âŠ™-assoc : Associative _âŠ™_
âŠ™-assoc x y z i .fst k = x .fst (y .fst (z .fst k))
âŠ™-assoc x y z i .snd k = squash (((x âŠ™ y) âŠ™ z) .snd k) ((x âŠ™ (y âŠ™ z)) .snd k) i

â“”âŠ™ : âˆ€ x â†’ â“” âŠ™ x â‰¡ x
â“”âŠ™ x i .fst y = x .fst y
â“”âŠ™ x i .snd y = squash ((â“” âŠ™ x) .snd y) (x .snd y) i

âŠ™â“” : âˆ€ x â†’ x âŠ™ â“” â‰¡ x
âŠ™â“” x i .fst y = x .fst y
âŠ™â“” x i .snd y = squash ((x âŠ™ â“”) .snd y) (x .snd y) i

cayleyMonoid : Monoid a
Monoid.ğ‘† cayleyMonoid = ğ’
Monoid._âˆ™_ cayleyMonoid = _âŠ™_
Monoid.Îµ cayleyMonoid = â“”
Monoid.assoc cayleyMonoid = âŠ™-assoc
Monoid.Îµâˆ™ cayleyMonoid = â“”âŠ™
Monoid.âˆ™Îµ cayleyMonoid = âŠ™â“”

open import Data.Sigma.Properties

module _ (sIsSet : isSet ğ‘†) where
  ğ’-leftInv-fst : âˆ€ x y â†’ âŸ¦ âŸ¦ x â‡“âŸ§ â‡‘âŸ§ .fst y â‰¡ x .fst y
  ğ’-leftInv-fst x y = rec (sIsSet (x .fst Îµ âˆ™ y) (x .fst y)) id (x .snd y)

  ğ’-leftInv : âˆ€ x â†’ âŸ¦ âŸ¦ x â‡“âŸ§ â‡‘âŸ§ â‰¡ x
  ğ’-leftInv x = Î£â‰¡Prop (Î» f xs ys â†’ funExt Î» x â†’ squash (xs x) (ys x)) (funExt (ğ’-leftInv-fst x))

  ğ’-iso : ğ’ â‡” ğ‘†
  fun ğ’-iso = âŸ¦_â‡“âŸ§
  inv ğ’-iso = âŸ¦_â‡‘âŸ§
  rightInv ğ’-iso = âˆ™Îµ
  leftInv ğ’-iso = ğ’-leftInv
